docs/03-formal-verification/easycrypt/ms/source/SourceCouplingTheorem.ec
@@ -1,0 +1,85 @@
+require import AllCore List Distr.
+require import QssmTypes.
+require import SourceTypes.
+require import SourcePayloadDistributions.
+require export SourceCouplingTypes.
+require import SourceConstructors.
+
+(* Marginal equalities for the product seed coupling (MS-3c parallel:
+   `ComparisonCouplingMarginals.ec`, lemmas `L_dmap_dprod_fst_lossless` /
+   `L_dmap_dprod_snd_lossless`). *)
+
+lemma L_dmap_dprod_fst_lossless_src ['a 'b] (da : 'a distr) (db : 'b distr) :
+  is_lossless db =>
+  dmap (da `*` db) fst = da.
+proof.
+move=> Hll.
+rewrite (dprod_marginalL da db (fun (a : 'a) => a)).
+rewrite dmap_id.
+have Hw: weight db = 1%r by apply (is_losslessP _ Hll).
+rewrite Hw dscalar1.
+by [].
+qed.
+
+lemma L_dmap_dprod_snd_lossless_src ['a 'b] (da : 'a distr) (db : 'b distr) :
+  is_lossless da =>
+  dmap (da `*` db) snd = db.
+proof.
+move=> Hll.
+rewrite (dprod_marginalR da db (fun (b : 'b) => b)).
+rewrite dmap_id.
+have Hw: weight da = 1%r by apply (is_losslessP _ Hll).
+rewrite Hw dscalar1.
+by [].
+qed.
+
+lemma L_ms3a_coupling_seed_real_projection_eq (x : ms_public_input) (s : seed) :
+  is_lossless (d_ms3a_sim_payload_seed x s) =>
+  d_ms3a_coupling_seed_real_projection x s = d_ms3a_real_payload_seed x.
+proof.
+move=> Hll.
+rewrite /d_ms3a_coupling_seed_real_projection /d_ms3a_real_sim_payload_seed_coupling.
+exact (L_dmap_dprod_fst_lossless_src (d_ms3a_real_payload_seed x) (d_ms3a_sim_payload_seed x s) Hll).
+qed.
+
+lemma L_ms3a_coupling_seed_sim_projection_eq (x : ms_public_input) (s : seed) :
+  is_lossless (d_ms3a_real_payload_seed x) =>
+  d_ms3a_coupling_seed_sim_projection x s = d_ms3a_sim_payload_seed x s.
+proof.
+move=> Hll.
+rewrite /d_ms3a_coupling_seed_sim_projection /d_ms3a_real_sim_payload_seed_coupling.
+exact (L_dmap_dprod_snd_lossless_src (d_ms3a_real_payload_seed x) (d_ms3a_sim_payload_seed x s) Hll).
+qed.
+
+lemma L_ms3a_coupling_seed_mem_components (x : ms_public_input) (s : seed)
+  (sr : ms3a_real_payload_seed) (ss : ms3a_sim_payload_seed) :
+  (sr, ss) \in d_ms3a_real_sim_payload_seed_coupling x s =>
+  sr \in d_ms3a_real_payload_seed x /\
+  ss \in d_ms3a_sim_payload_seed x s.
+proof.
+move=> Hmem.
+rewrite /d_ms3a_real_sim_payload_seed_coupling in Hmem.
+rewrite supp_dprod in Hmem.
+by case: Hmem.
+qed.
+
+lemma L_ms3a_real_sim_payload_seed_coupled_layer_maps_eq
+  (sr : ms3a_real_payload_seed) (ss : ms3a_sim_payload_seed) :
+  ms3a_real_sim_payload_seed_coupled sr ss =>
+  ms3a_bitness_layer_source_of_real_payload sr =
+  ms3a_bitness_layer_source_of_sim_payload ss.
+proof.
+move=> [Hpub [Hbits [Htd _]]].
+have [Hstmt [Hres [Hcomp Hbg]]] := Hpub.
+rewrite /ms3a_bitness_layer_source_of_real_payload /ms3a_bitness_layer_source_of_sim_payload
+  /ms3a_make_real_source /ms3a_make_sim_source.
+by rewrite Hstmt Hres Hbits Hbg Hcomp Htd.
+qed.
+
+lemma L_ms3a_real_sim_payload_seed_coupled_implies_public_match
+  (sr : ms3a_real_payload_seed) (ss : ms3a_sim_payload_seed) :
+  ms3a_real_sim_payload_seed_coupled sr ss =>
+  ms3a_payload_pair_public_fields_match sr ss.
+proof.
+by move=> [Hpub _].
+qed.
