docs/03-formal-verification/easycrypt/ms/source/SourcePublicFieldObligations.ec
@@ -5,6 +5,58 @@ require import SourceProgrammedObligations.
 
 (* Paired public-field seed axioms, `from_seed` lemmas, and payload-support programming. *)
 
+(* Phase-1 spine linkage: if joint support seeds equal the Phase-1 constructors, the four
+   field equalities in `A_ms3a_seed_pair_*_source_shared` follow without those axioms. The
+   unconditional axioms remain until `d_ms3a_*_payload_seed` is refined to enforce this. *)
+
+lemma L_ms3a_seed_pair_stmt_when_seeds_are_phase1
+  (x : ms_public_input) (s : seed) (sr : ms3a_real_payload_seed) (ss : ms3a_sim_payload_seed) :
+  sr \in d_ms3a_real_payload_seed x =>
+  ss \in d_ms3a_sim_payload_seed x s =>
+  sr = ms3a_phase1_real_payload_from_public_input x =>
+  ss = ms3a_phase1_sim_payload_from_public_input x =>
+  sr.`ms3rp_stmt = ss.`ms3sp_stmt.
+proof.
+move=> _ _ -> ->.
+by rewrite /ms3a_phase1_real_payload_from_public_input /ms3a_phase1_sim_payload_from_public_input.
+qed.
+
+lemma L_ms3a_seed_pair_res_when_seeds_are_phase1
+  (x : ms_public_input) (s : seed) (sr : ms3a_real_payload_seed) (ss : ms3a_sim_payload_seed) :
+  sr \in d_ms3a_real_payload_seed x =>
+  ss \in d_ms3a_sim_payload_seed x s =>
+  sr = ms3a_phase1_real_payload_from_public_input x =>
+  ss = ms3a_phase1_sim_payload_from_public_input x =>
+  sr.`ms3rp_res = ss.`ms3sp_res.
+proof.
+move=> _ _ -> ->.
+by rewrite /ms3a_phase1_real_payload_from_public_input /ms3a_phase1_sim_payload_from_public_input.
+qed.
+
+lemma L_ms3a_seed_pair_comparison_global_when_seeds_are_phase1
+  (x : ms_public_input) (s : seed) (sr : ms3a_real_payload_seed) (ss : ms3a_sim_payload_seed) :
+  sr \in d_ms3a_real_payload_seed x =>
+  ss \in d_ms3a_sim_payload_seed x s =>
+  sr = ms3a_phase1_real_payload_from_public_input x =>
+  ss = ms3a_phase1_sim_payload_from_public_input x =>
+  sr.`ms3rp_comparison_global_challenge = ss.`ms3sp_comparison_global_challenge.
+proof.
+move=> _ _ -> ->.
+by rewrite /ms3a_phase1_real_payload_from_public_input /ms3a_phase1_sim_payload_from_public_input.
+qed.
+
+lemma L_ms3a_seed_pair_bitness_globals_when_seeds_are_phase1
+  (x : ms_public_input) (s : seed) (sr : ms3a_real_payload_seed) (ss : ms3a_sim_payload_seed) :
+  sr \in d_ms3a_real_payload_seed x =>
+  ss \in d_ms3a_sim_payload_seed x s =>
+  sr = ms3a_phase1_real_payload_from_public_input x =>
+  ss = ms3a_phase1_sim_payload_from_public_input x =>
+  sr.`ms3rp_bitness_global_challenges = ss.`ms3sp_bitness_global_challenges.
+proof.
+move=> _ _ -> ->.
+by rewrite /ms3a_phase1_real_payload_from_public_input /ms3a_phase1_sim_payload_from_public_input.
+qed.
+
 axiom A_ms3a_seed_pair_stmt_source_shared (x : ms_public_input) (s : seed) :
   forall (sr : ms3a_real_payload_seed) (ss : ms3a_sim_payload_seed),
     sr \in d_ms3a_real_payload_seed x =>
